theories/GHC/iS4_Lindenbaum_lem.v
@@ -17,17 +17,8 @@ Section Sets_of_forms.
 
 Definition SubTheory (Γ Δ : @Ensemble form) (Incl: Included _ Δ Γ) := forall φ, (iS4H_prv (Δ, φ) /\ In _ Γ φ) -> In _ Δ φ.
 
-(* Definition closed Γ :=
-  forall φ, iS4H_rules (Γ, φ) -> Γ φ. *)
-
 Definition restr_closed Γ Δ :=
   forall φ, iS4H_rules (Δ, φ) -> Γ φ -> Δ φ.
-
-(* Definition stable (Γ : @Ensemble form) :=
-  forall φ, ~ ~ Γ φ -> Γ φ. *)
-
-Definition restr_stable (Γ Δ  : @Ensemble form) :=
-  forall φ, Γ φ -> ~ ~ Δ φ -> Δ φ.
 
 Definition prime (Γ : @Ensemble form) :=
   forall φ ψ, Γ (Or φ ψ) -> Γ φ \/ Γ ψ.
@@ -385,124 +376,6 @@ remember (form_index a) as n. destruct n ; simpl.
      inversion H4 ; subst. 2: inversion H5. apply Id. apply IdRule_I ; auto.
 Qed.
 
-Lemma quasi_prime_Lind_theory': forall Γ Δ ψ,
-  Included _ Δ (Clos' Γ) ->
-  ~ iS4H_prv (Δ, ψ) ->
-  quasi_prime (Lind_theory (Clos' Γ) Δ ψ).
-Proof.
-intros Γ Δ ψ Incl H0 a b Hor H1. remember (Clos' Γ) as CΓ.
-
-apply H1. left. exists (form_index a).
-remember (form_index a) as n. destruct n ; simpl.
-- unfold choice_code. unfold choice_form. unfold In.
-  right. repeat split. 3: rewrite Heqn ; apply form_enum_index.
-  subst. apply Incl_ClosSubform_Clos'. exists (a ∨ b). split ; auto.
-  apply incl_Lind_theory in Hor ; auto.
-  simpl. right ; apply in_or_app ; left ; destruct a ; simpl ; auto.
-  intro. apply H1. right. exists (form_index b).
-  remember (form_index b) as m. destruct m ; simpl.
-  + rewrite Heqm in Heqn. apply form_index_inj in Heqn.
-     subst. exfalso.
-     pose (Under_Lind_theory (Clos' Γ) Δ ψ Incl H0). apply n.
-    apply MP with (ps:=[(Lind_theory (Clos' Γ) Δ ψ, (Or a a) --> ψ);
-    (Lind_theory (Clos' Γ) Δ ψ, (Or a a))]). 2: apply MPRule_I. intros. inversion H2 ; subst.
-    apply MP with (ps:=[(Lind_theory (Clos' Γ) Δ ψ, (a --> ψ) --> (Or a a --> ψ));
-    (Lind_theory (Clos' Γ) Δ ψ, (a --> ψ))]). 2: apply MPRule_I. intros. inversion H3 ; subst.
-    apply MP with (ps:=[(Lind_theory (Clos' Γ) Δ ψ, (a --> ψ) --> (a --> ψ) --> (Or a a --> ψ));
-    (Lind_theory (Clos' Γ) Δ ψ, (a --> ψ))]). 2: apply MPRule_I. intros. inversion H4 ; subst.
-    apply Ax. apply AxRule_I. left. apply IA5_I. exists a. exists a. exists ψ. auto.
-    inversion H5 ; subst. 2: inversion H6.
-    apply iS4H_Deduction_Theorem with (s:=(Union (form) (Lind_theory (Clos' Γ) Δ ψ) (Singleton (form) a), ψ)) ; auto.
-    apply iS4H_monot with (Γ1:=Union form (Lind_theory (Clos' Γ) Δ ψ) (Singleton form a)) in H ; auto.
-    simpl ; intros c Hc. inversion Hc ; subst. apply Union_introl. apply Lind_theory_extens ; auto.
-    inversion H6 ; subst ; apply Union_intror ; apply In_singleton.
-    inversion H4 ; subst. 2: inversion H5.
-    apply iS4H_Deduction_Theorem with (s:=(Union (form) (Lind_theory (Clos' Γ) Δ ψ) (Singleton (form) a), ψ)) ; auto.
-    apply iS4H_monot with (Γ1:=Union form (Lind_theory (Clos' Γ) Δ ψ) (Singleton form a)) in H ; auto.
-    simpl ; intros c Hc. inversion Hc ; subst. apply Union_introl. apply Lind_theory_extens ; auto.
-    inversion H5 ; subst ; apply Union_intror ; apply In_singleton.
-    inversion H3 ; subst. 2: inversion H4. apply Id. apply IdRule_I ; auto.
-  + subst. unfold choice_code. unfold choice_form. unfold In. right. repeat split.
-     subst. apply Incl_ClosSubform_Clos'. exists (a ∨ b). split ; auto.
-     apply incl_Lind_theory in Hor ; auto.
-     simpl. right ; apply in_or_app ; right ; destruct b ; simpl ; auto.
-     2: rewrite Heqm ; apply form_enum_index. intro.
-     pose (Under_Lind_theory (Clos' Γ) Δ ψ Incl H0). apply n.
-     apply MP with (ps:=[(Lind_theory (Clos' Γ) Δ ψ, (Or a b) --> ψ);
-     (Lind_theory (Clos' Γ) Δ ψ, (Or a b))]). 2: apply MPRule_I. intros. inversion H3 ; subst.
-     apply MP with (ps:=[(Lind_theory (Clos' Γ) Δ ψ, (b --> ψ) --> (Or a b --> ψ));
-     (Lind_theory (Clos' Γ) Δ ψ, (b --> ψ))]). 2: apply MPRule_I. intros. inversion H4 ; subst.
-     apply MP with (ps:=[(Lind_theory (Clos' Γ) Δ ψ, (a --> ψ) --> (b --> ψ) --> (Or a b --> ψ));
-     (Lind_theory (Clos' Γ) Δ ψ, (a --> ψ))]). 2: apply MPRule_I. intros. inversion H5 ; subst.
-     apply Ax. apply AxRule_I. left. apply IA5_I. exists a. exists b. exists ψ. auto.
-     inversion H6 ; subst. 2: inversion H7.
-     apply iS4H_Deduction_Theorem with (s:=(Union (form) (Lind_theory (Clos' Γ) Δ ψ) (Singleton (form) a), ψ)) ; auto.
-     apply iS4H_monot with (Γ1:=Union form (Lind_theory (Clos' Γ) Δ ψ) (Singleton form a)) in H ; auto.
-     simpl ; intros c Hc. inversion Hc ; subst. apply Union_introl. apply Lind_theory_extens ; auto.
-     inversion H7 ; subst ; apply Union_intror ; apply In_singleton.
-     inversion H5 ; subst. 2: inversion H6.
-     apply iS4H_Deduction_Theorem with (s:=(Union (form) (Lind_theory (Clos' Γ) Δ ψ) (Singleton (form) b), ψ)) ; auto.
-     apply iS4H_monot with (Γ1:=Union form (Lind_theory (Clos' Γ) Δ ψ) (Singleton form b)) in H2 ; auto.
-     simpl ; intros c Hc. inversion Hc ; subst. apply Union_introl. unfold In. exists m ; auto.
-     inversion H6 ; subst ; apply Union_intror ; apply In_singleton.
-     inversion H4 ; subst. 2: inversion H5. apply Id. apply IdRule_I ; auto.
-- unfold choice_code. unfold choice_form. unfold In.
-  right. repeat split. 3: rewrite Heqn ; apply form_enum_index.
-  subst. apply Incl_ClosSubform_Clos'. exists (a ∨ b). split ; auto.
-  apply incl_Lind_theory in Hor ; auto.
-  simpl. right ; apply in_or_app ; left ; destruct a ; simpl ; auto.
-  intro. apply H1. right. exists (form_index b).
-  remember (form_index b) as m. destruct m ; simpl.
-  + subst. unfold choice_code. unfold choice_form. unfold In. right. repeat split.
-     subst. apply Incl_ClosSubform_Clos'. exists (a ∨ b). split ; auto.
-     apply incl_Lind_theory in Hor ; auto.
-     simpl. right ; apply in_or_app ; right ; destruct b ; simpl ; auto.
-     2: rewrite Heqm ; apply form_enum_index. intro.
-     pose (Under_Lind_theory (Clos' Γ) Δ ψ Incl H0). apply n0.
-     apply MP with (ps:=[(Lind_theory (Clos' Γ) Δ ψ, (Or a b) --> ψ);
-     (Lind_theory (Clos' Γ) Δ ψ, (Or a b))]). 2: apply MPRule_I. intros. inversion H3 ; subst.
-     apply MP with (ps:=[(Lind_theory (Clos' Γ) Δ ψ, (b --> ψ) --> (Or a b --> ψ));
-     (Lind_theory (Clos' Γ) Δ ψ, (b --> ψ))]). 2: apply MPRule_I. intros. inversion H4 ; subst.
-     apply MP with (ps:=[(Lind_theory (Clos' Γ) Δ ψ, (a --> ψ) --> (b --> ψ) --> (Or a b --> ψ));
-     (Lind_theory (Clos' Γ) Δ ψ, (a --> ψ))]). 2: apply MPRule_I. intros. inversion H5 ; subst.
-     apply Ax. apply AxRule_I. left. apply IA5_I. exists a. exists b. exists ψ. auto.
-     inversion H6 ; subst. 2: inversion H7.
-     apply iS4H_Deduction_Theorem with (s:=(Union (form) (Lind_theory (Clos' Γ) Δ ψ) (Singleton (form) a), ψ)) ; auto.
-     apply iS4H_monot with (Γ1:=Union form (Lind_theory (Clos' Γ) Δ ψ) (Singleton form a)) in H ; auto.
-     simpl ; intros c Hc. inversion Hc ; subst. apply Union_introl. unfold In ; exists n ; auto.
-     inversion H7 ; subst ; apply Union_intror ; apply In_singleton.
-     inversion H5 ; subst. 2: inversion H6.
-     apply iS4H_Deduction_Theorem with (s:=(Union (form) (Lind_theory (Clos' Γ) Δ ψ) (Singleton (form) b), ψ)) ; auto.
-     apply iS4H_monot with (Γ1:=Union form (Lind_theory (Clos' Γ) Δ ψ) (Singleton form b)) in H2 ; auto.
-     simpl ; intros c Hc. inversion Hc ; subst. apply Union_introl. apply Lind_theory_extens ; auto.
-     inversion H6 ; subst ; apply Union_intror ; apply In_singleton.
-     inversion H4 ; subst. 2: inversion H5. apply Id. apply IdRule_I ; auto.
-  + subst. unfold choice_code. unfold choice_form. unfold In. right. repeat split.
-     subst. apply Incl_ClosSubform_Clos'. exists (a ∨ b). split ; auto.
-     apply incl_Lind_theory in Hor ; auto.
-     simpl. right ; apply in_or_app ; right ; destruct b ; simpl ; auto.
-     2: rewrite Heqm ; apply form_enum_index. intro.
-     pose (Under_Lind_theory (Clos' Γ) Δ ψ Incl H0). apply n0.
-     apply MP with (ps:=[(Lind_theory (Clos' Γ) Δ ψ, (Or a b) --> ψ);
-     (Lind_theory (Clos' Γ) Δ ψ, (Or a b))]). 2: apply MPRule_I. intros. inversion H3 ; subst.
-     apply MP with (ps:=[(Lind_theory (Clos' Γ) Δ ψ, (b --> ψ) --> (Or a b --> ψ));
-     (Lind_theory (Clos' Γ) Δ ψ, (b --> ψ))]). 2: apply MPRule_I. intros. inversion H4 ; subst.
-     apply MP with (ps:=[(Lind_theory (Clos' Γ) Δ ψ, (a --> ψ) --> (b --> ψ) --> (Or a b --> ψ));
-     (Lind_theory (Clos' Γ) Δ ψ, (a --> ψ))]). 2: apply MPRule_I. intros. inversion H5 ; subst.
-     apply Ax. apply AxRule_I. left. apply IA5_I. exists a. exists b. exists ψ. auto.
-     inversion H6 ; subst. 2: inversion H7.
-     apply iS4H_Deduction_Theorem with (s:=(Union (form) (Lind_theory (Clos' Γ) Δ ψ) (Singleton (form) a), ψ)) ; auto.
-     apply iS4H_monot with (Γ1:=Union form (Lind_theory (Clos' Γ) Δ ψ) (Singleton form a)) in H ; auto.
-     simpl ; intros c Hc. inversion Hc ; subst. apply Union_introl. unfold In. exists n ; auto.
-     inversion H7 ; subst ; apply Union_intror ; apply In_singleton.
-     inversion H5 ; subst. 2: inversion H6.
-     apply iS4H_Deduction_Theorem with (s:=(Union (form) (Lind_theory (Clos' Γ) Δ ψ) (Singleton (form) b), ψ)) ; auto.
-     apply iS4H_monot with (Γ1:=Union form (Lind_theory (Clos' Γ) Δ ψ) (Singleton form b)) in H2 ; auto.
-     simpl ; intros c Hc. inversion Hc ; subst. apply Union_introl. unfold In. exists m ; auto.
-     inversion H6 ; subst ; apply Union_intror ; apply In_singleton.
-     inversion H4 ; subst. 2: inversion H5. apply Id. apply IdRule_I ; auto.
-Qed.
-
 (* A prime pair is consistent. *)
 
 Lemma Consist_nLind_theory : forall n Γ Δ ψ,
@@ -529,30 +402,6 @@ apply MP with (ps:=[(Lind_theory Γ Δ ψ, Bot --> ψ);(Lind_theory Γ Δ ψ, Bo
 inversion H4.
 Qed.
 
-(* A prime set is stable. *)
-
-Lemma stable_Lind_theory: forall Γ Δ ψ,
-  Included _ Δ Γ ->
-  ~ iS4H_prv (Δ, ψ) ->
-  restr_stable Γ (Lind_theory Γ Δ ψ).
-Proof.
-intros Γ Δ ψ Incl H a Ha H0. exists (form_index a).
-unfold nLind_theory. simpl. unfold In.
-remember (form_index a) as n. pose (form_enum_index a). destruct n.
--  unfold choice_code. unfold choice_form. right ; repeat split ; subst ; auto.
-   intro. apply H0. intro.
-   apply Under_Lind_theory with (Γ:=Γ) (Δ:=Δ) (ψ:=ψ) ; auto.
-   apply iS4H_monot with (Γ1:=(Lind_theory Γ Δ ψ)) in H1 ; auto.
-   intro. simpl ; intros. inversion H3 ; subst. apply Lind_theory_extens ; auto.
-   inversion H4 ; subst ; auto. rewrite <- Heqn in e. rewrite e. auto.
--  unfold choice_code. unfold choice_form. right ; repeat split ; auto.
-   intro. apply H0. intro.
-   apply Under_Lind_theory with (Γ:=Γ) (Δ:=Δ) (ψ:=ψ) ; auto.
-   apply iS4H_monot with (Γ1:=(Lind_theory Γ Δ ψ)) in H1 ; auto.
-   simpl ; intro. simpl ; intros. inversion H3 ; subst. exists n ; auto.
-   inversion H4 ; subst ; auto. rewrite <- Heqn in e. rewrite e. auto.
-Qed.
-
 End PrimeProps.
 
 
@@ -569,7 +418,6 @@ Lemma Lindenbaum Γ Δ ψ :
   exists Δm, Included _ Δ Δm
            /\ Included _ Δm (Clos Γ)
            /\ restr_closed (Clos Γ) Δm
-           /\ restr_stable (Clos Γ) Δm
            /\ quasi_prime Δm
            /\ ~ iS4H_prv (Δm, ψ).
 Proof.
@@ -579,31 +427,8 @@ repeat split.
 - intro. apply Lind_theory_extens.
 - apply incl_Lind_theory ; auto.
 - apply restr_closeder_Lind_theory ; auto.
-- apply stable_Lind_theory ; auto.
 - pose quasi_prime_Lind_theory ; auto.
 - intro. apply Under_Lind_theory with (Γ:=(Clos Γ)) in H1 ; auto.
-Qed.
-
-Lemma Lindenbaum' Γ Δ ψ :
-  In _ (Clos' Γ) ψ ->
-  Included _ Δ (Clos' Γ) ->
-  ~ iS4H_prv (Δ, ψ) ->
-  exists Δm, Included _ Δ Δm
-           /\ Included _ Δm (Clos' Γ)
-           /\ restr_closed (Clos' Γ) Δm
-           /\ restr_stable (Clos' Γ) Δm
-           /\ quasi_prime Δm
-           /\ ~ iS4H_prv (Δm, ψ).
-Proof.
-intros.
-exists (Lind_theory (Clos' Γ) Δ ψ).
-repeat split.
-- intro. apply Lind_theory_extens.
-- apply incl_Lind_theory ; auto.
-- apply restr_closeder_Lind_theory ; auto.
-- apply stable_Lind_theory ; auto.
-- pose quasi_prime_Lind_theory' ; auto.
-- intro. apply Under_Lind_theory with (Γ:=(Clos' Γ)) in H1 ; auto.
 Qed.
 
 End Lindenbaum.
